IcTheory/Compression.lean
@@ -8,3 +8,4 @@ import IcTheory.Compression.Theorem33
 import IcTheory.Compression.Corollary31
 import IcTheory.Compression.Theorem34
 import IcTheory.Compression.Theorem36
+import IcTheory.Compression.Theorem35
